getting somewhere

core/main.v
@@ -1,92 +1,147 @@
 Add LoadPath "/home/blaine/lab/cpdtlib" as Cpdt.
 Set Implicit Arguments. Set Asymmetric Patterns.
-Require Import List String Cpdt.CpdtTactics.
-Import ListNotations. Open Scope string_scope.
+Require Import List.
+Import ListNotations.
+Open Scope list_scope.
+Require String.
+Require Import Cpdt.CpdtTactics.
+Require Import Lt.
 
 Require Import core.utils.
 
-Inductive BaseModifier: Set :=
-	| Many
-	| Maybe
-	| MaybeMany
-.
 
+Inductive BaseModifier: Set :=
+	(*| Many*)
+	| Maybe
+	(*| MaybeMany*)
+.
 Definition Modifier := option BaseModifier.
 
-Definition Modifier_is_optional(modifier: Modifier): bool :=
+Definition ModifierOptional (modifier: Modifier): Prop := modifier = Some Maybe.
+Definition ModifierOptionalBool modifier :=
+	{ModifierOptional modifier} + {~(ModifierOptional modifier)}.
+Obligation Tactic := crush.
+Program Definition Modifier_optional modifier: ModifierOptionalBool modifier :=
 	match modifier with
 	| Some m => match m with
-		| Many => false
-		| Maybe => true
-		| MaybeMany => true
+		(*| Many => No*)
+		| Maybe => Yes
+		(*| MaybeMany => Yes*)
 		end
-	| None => false
+	| None => No
 	end.
 
 
-Definition TokenDefinition := string.
-Definition Token := string.
-(*Definition token_definition_precludes := string_dec.*)
+Definition TokenDefinition := String.string.
+Definition Token := String.string.
 
-Definition TokenMatchesProp (def: TokenDefinition) (token: Token): Prop := def = token.
-Definition TokenMatches def token :=
-	{TokenMatchesProp def token} + {~(TokenMatchesProp def token)}.
-
+Definition TokenMatches (def: TokenDefinition) (token: Token): Prop := def = token.
+Definition TokenMatchesBool def token :=
+	{TokenMatches def token} + {~(TokenMatches def token)}.
 Obligation Tactic := crush.
-Program Definition match_token def token: TokenMatches def token :=
-	Reduce (string_dec def token).
+Program Definition match_token def token: TokenMatchesBool def token :=
+	Reduce (String.string_dec def token).
 
 
-Inductive TokensMatchProp: list TokenDefinition -> list Token -> Prop :=
-	| TokensMatchProp_base:
-		forall def token, TokenMatchesProp def token
-			-> TokensMatchProp [def] [token]
-	| TokensMatchProp_append:
-		forall defs tokens def token, TokensMatchProp defs tokens -> TokenMatchesProp def token
-			-> TokensMatchProp (def :: defs) (token :: tokens)
+Definition TokenPath := list TokenDefinition.
+Definition TokenStream := list Token.
+
+Inductive PathMatchesStream: TokenPath -> TokenStream -> Prop :=
+	| PathMatchesStream_base: forall def token,
+		TokenMatches def token
+		-> PathMatchesStream [def] [token]
+	| PathMatchesStream_append: forall def token path stream,
+		TokenMatches def token
+		-> PathMatchesStream path stream
+		-> PathMatchesStream (def :: path) (token :: stream)
 .
-Hint Constructors TokensMatchProp: core.
-Definition TokensMatch defs tokens :=
-  {TokensMatchProp defs tokens} + {~(TokensMatchProp defs tokens)}.
+Hint Constructors PathMatchesStream: core.
 
-(*Obligation Tactic := crush.
-Program Fixpoint match_tokens defs tokens: TokensMatch defs tokens :=
-	match defs, tokens with
-	| def :: defs', token :: tokens' => if match_token def token
-		then Reduce (match_tokens defs' tokens')
-		else No
-	| _, _ => No
+Theorem PathMatchesStream_neither_empty:
+	forall path stream, PathMatchesStream path stream -> path <> [] /\ stream <> [].
+Proof. intros p s m. inversion m; crush. Qed.
+Hint Resolve PathMatchesStream_neither_empty: core.
+
+Theorem PathMatchesStream_length_non_zero:
+	forall path stream, PathMatchesStream path stream -> 0 < (length path) /\ 0 < (length stream).
+Proof. intros p s m. inversion m; crush. Qed.
+Hint Resolve PathMatchesStream_length_non_zero: core.
+
+
+Inductive Node: Type :=
+	| consume (modifier: Modifier) (defs: NonEmpty TokenDefinition)
+.
+Definition Node_modifier (node: Node): Modifier :=
+	match node with
+	| consume modifier _ => modifier
 	end.
+Hint Unfold Node_modifier: core.
+
+Inductive NodeMatchesStream: Node -> TokenStream -> Prop :=
+	| NodeMatchesStream_consume_required: forall modifier defs stream,
+		PathMatchesStream (listOf defs) stream
+		-> NodeMatchesStream (consume modifier defs) stream
+	| NodeMatchesStream_consume_optional: forall modifier defs,
+		ModifierOptional modifier
+		-> NodeMatchesStream (consume modifier defs) []
+.
+Hint Constructors NodeMatchesStream: core.
+
+Theorem Node_non_optional_stream_not_empty:
+	forall node stream,
+		~(ModifierOptional (Node_modifier node))
+		-> NodeMatchesStream node stream
+		-> stream <> [].
+Proof. intros n s r ma. inversion ma; crush; inversion H. Qed.
+Hint Resolve Node_non_optional_stream_not_empty: core.
+
+Theorem Node_non_optional_length_non_zero:
+	forall node stream,
+		~(ModifierOptional (Node_modifier node))
+		-> NodeMatchesStream node stream
+		-> 0 < (length stream).
+Proof. intros n s r ma. inversion ma; inversion H; crush. Qed.
+Hint Resolve Node_non_optional_stream_not_empty: core.
+
+Inductive NodeListMatchesStream: list Node -> TokenStream -> Prop :=
+	| NodeListMatchesStream_base: forall node stream,
+		NodeMatchesStream node stream
+		-> NodeListMatchesStream [node] stream
+	| NodeListMatchesStream_append: forall node stream nodes streams,
+		NodeMatchesStream node stream
+		-> NodeListMatchesStream nodes streams
+		-> NodeListMatchesStream (node :: nodes) (app stream streams)
+.
+Hint Constructors NodeListMatchesStream: core.
+
+(*what's maybe more interesting here is that if you add a non-optional node to any list of nodes, the length of the match will only increase and not merely remain the same*)
+
+Theorem Node_add_non_optional_increases_match_length:
+	forall node stream nodes streams,
+		~(ModifierOptional (Node_modifier node))
+		-> NodeListMatchesStream (node :: nodes) (app stream streams)
+		-> (length streams) < (length (stream ++ streams)).
+Proof.
+	intros n s ns ss r ma. inversion ma; crush. inversion H2; crush. inversion H; crush.
+Qed.
+
+
+(*
+now it's all about how to define a "maximal" match
+that's what defines a correct lookahead, it will tell us whether to take the current option in such a way that the overall match we produce will be maximal
+now just what is maximal????
 *)
 
-Theorem TokensMatchProp_same_not_empty:
-	forall defs tokens, TokensMatchProp defs tokens -> defs <> [] /\ tokens <> [].
-Proof.
-	intros d t m. induction m; crush.
-Qed.
-Hint Resolve TokensMatchProp_same_not_empty: core.
-Theorem TokenMatchesProp_not_if_empty:
-	forall defs tokens, defs = [] \/ tokens = [] -> ~(TokensMatchProp defs tokens).
-Proof.
-	intros d t [dn|tn] m; induction m; crush.
-Qed.
-Hint Resolve TokenMatchesProp_not_if_empty: core.
 
-Definition match_tokens: forall defs tokens, TokensMatch defs tokens.
-	refine (fix match_tokens_recursive defs tokens: TokensMatch defs tokens :=
-		match defs, tokens with
-		| [def], [token] => Reduce (match_token def token)
-		| def :: defs', token :: tokens' => if match_token def token
-			then Reduce (match_tokens_recursive defs' tokens')
-			else No
-		| _, _ => No
-		end
-	); try (apply TokensMatchProp_base; crush); try (intros m; inversion m; crush).
-	-
-Defined.
+(*
+
+let's say we have a rule like this that we need to generate lookaheads for
+what we really want to know is what lookahead do we need to test when we hit A B
+a consume is all or nothing
+(A B)? (A)
+
+the lookahead has to be (A B), since merely (A) would falsely enter the ? consume if the
 
 
-Record Consume: Type := consume {
-	tokens: NonEmpty TokenDefinition,
-}.
+*)
 
