scratch.v
@@ -1,0 +1,115 @@
+Definition ModifierMany (modifier: Modifier): Prop := modifier = Some Many /\ modifier = Some MaybeMany.
+Definition ModifierManyBool :=
+	{ModifierMany modifier} + {~(ModifierMany modifier)}.
+Obligation Tactic := crush.
+Program Definition Modifier_many modifier: ModifierManyBool modifier :=
+	match modifier with
+	| Some m => match m with
+		| Many => Yes
+		| Maybe => No
+		| MaybeMany => Yes
+		end
+	| None => No
+	end.
+
+
+(*
+| ConsumeMatchesStream_many_consume: forall modifier defs stream,
+		ModifierMany modifier
+		-> PathMatchesStream (listOf defs) stream
+		-> ConsumeMatchesStream (consume modifier defs) (app stream stream)
+*)
+
+
+
+
+
+
+Inductive PathMatches: TokenPath -> TokenStream -> TokenStream -> Prop :=
+	| PathMatches_base: forall def token,
+		TokenMatchesProp def token
+		-> forall remainder, PathMatches [def] (token :: remainder) [token]
+	| PathMatches_append: forall def token,
+		TokenMatchesProp def token
+		-> forall path stream remainder, PathMatches path (stream ++ remainder)%list stream
+		-> PathMatches (def :: path) (token :: (stream ++ remainder)%list) (token :: stream)
+.
+Hint Constructors PathMatches: core.
+
+(*Inductive PathMatchesFront: TokenPath -> TokenStream -> TokenStream -> Prop :=
+	| PathMatchesFront_all: forall path stream,
+		PathMatches path stream
+		-> forall remainder, PathMatchesFront path (stream ++ remainder) stream
+.*)
+
+
+Inductive Node: Type :=
+	| Consume (modifier: Modifier) (defs: NonEmpty TokenDefinition)
+	(*| Or (modifier: Modifier) (choices: NonLone (NonEmpty Node))*)
+	(*| Subrule (modifier: Modifier) (rule_name: string)*)
+	(*| MacroCall (modifier: Modifier) (macro_name: string) (args: NonEmpty (NonEmpty Node))*)
+	(*| Var (modifier: Modifier) (arg_name: string)*)
+	(*| LockingVar (modifier: Modifier) (locking_arg_name: string)*)
+	(*| Paren (modifier: BaseModifier) (nodes: NonLone Node)*)
+.
+
+(*Inductive GrammarItem: Type :=
+	| TokenDef (name: string)
+	| Rule (name: string) (definition: NonEmpty Node) (locking_args: list LockingArg)
+	| Macro (name: string) (args: NonEmpty Arg) (definition: NonEmpty Node) (locking_args: list LockingArg)
+	| VirtualLexerUsage (name path: string) (args: Regex?) (exposed_tokens: list string)
+.*)
+
+(*Fixpoint compute_lookahead (target against: TokenPath): Lookahead target against := .*)
+
+
+
+(*
+Inductive TokensMatchProp: list TokenDefinition -> list Token -> Prop :=
+	| TokensMatchProp_base:
+		forall def token, TokenMatchesProp def token
+			-> TokensMatchProp [def] [token]
+	| TokensMatchProp_append: forall defs tokens def token,
+		TokensMatchProp defs tokens
+		-> TokenMatchesProp def token
+			-> TokensMatchProp (def :: defs) (token :: tokens)
+.
+Hint Constructors TokensMatchProp: core.
+Definition TokensMatch defs tokens :=
+	{TokensMatchProp defs tokens} + {~(TokensMatchProp defs tokens)}.
+*)
+
+(*
+Theorem TokensMatchProp_same_not_empty:
+	forall defs tokens, TokensMatchProp defs tokens -> defs <> [] /\ tokens <> [].
+Proof.
+	intros d t m. induction m; crush.
+Qed.
+Hint Resolve TokensMatchProp_same_not_empty: core.
+Theorem TokenMatchesProp_not_if_empty:
+	forall defs tokens, defs = [] \/ tokens = [] -> ~(TokensMatchProp defs tokens).
+Proof.
+	intros d t [dn|tn] m; induction m; crush.
+Qed.
+Hint Resolve TokenMatchesProp_not_if_empty: core.
+*)
+
+(*
+Definition match_tokens: forall defs tokens, TokensMatch defs tokens.
+	refine (fix match_tokens_recursive defs tokens: TokensMatch defs tokens :=
+		match defs, tokens with
+		| [def], [token] => Reduce (match_token def token)
+		| def :: defs', token :: tokens' => if match_token def token
+			then Reduce (match_tokens_recursive defs' tokens')
+			else No
+		| _, _ => No
+		end
+	); try (apply TokensMatchProp_base; crush); try (intros m; inversion m; crush).
+	-
+Defined.
+
+
+Record Consume: Type := consume {
+	tokens: NonEmpty TokenDefinition,
+}.
+*)
